code/ecdsap256/Hacl.Impl.P256.ScalarMult.fsti
@@ -1,0 +1,36 @@
+module Hacl.Impl.P256.ScalarMult
+
+open FStar.HyperStack.All
+open FStar.HyperStack
+module ST = FStar.HyperStack.ST
+
+open Lib.IntTypes
+open Lib.Buffer
+
+open Spec.P256
+open Spec.ECDSA
+open Spec.P256.Definitions
+open Hacl.Spec.P256.Felem
+open Hacl.Impl.P256.Core
+
+open Spec.DH
+
+
+inline_for_extraction noextract
+val ecp256scalar_mult:
+    result:lbuffer uint8 (size 64)
+  -> pubKey:lbuffer uint8 (size 64)
+  -> scalar:lbuffer uint8 (size 32)
+  -> Stack bool
+    (requires fun h ->
+      live h result /\ live h pubKey /\ live h scalar /\
+      disjoint result pubKey /\ disjoint result scalar)
+    (ensures fun h0 r h1 ->
+      let pubKeyX = gsub pubKey (size 0) (size 32) in
+      let pubKeyY = gsub pubKey (size 32) (size 32) in
+      let pointX, pointY, flag =
+        ecp256_dh_r (as_seq h0 pubKeyX) (as_seq h0 pubKeyY) (as_seq h0 scalar) in
+      r == flag /\
+      modifies (loc result) h0 h1 /\
+      as_seq h1 (gsub result (size 0) (size 32)) == pointX /\
+      as_seq h1 (gsub result (size 32) (size 32)) == pointY)
